Manual/Coercions.lean
@@ -101,7 +101,7 @@ end
 #check Int.bdiv
 
 /--
-error: invalid field 'bdiv', the environment does not contain 'Nat.bdiv'
+error: Invalid field `bdiv`: The environment does not contain `Nat.bdiv`
   n
 has type
   Nat
@@ -122,7 +122,7 @@ The coercion from {lean}`Nat` to {lean}`Int` is not considered when looking up t
 example (n : Nat) := n.bdiv 2
 ```
 ```leanOutput natBdiv
-invalid field 'bdiv', the environment does not contain 'Nat.bdiv'
+Invalid field `bdiv`: The environment does not contain `Nat.bdiv`
   n
 has type
   Nat
@@ -221,7 +221,7 @@ numerals are polymorphic in Lean, but the numeral `9` cannot be used in a contex
   Bin
 due to the absence of the instance above
 
-Additional diagnostic information may be available using the `set_option diagnostics true` command.
+Hint: Additional diagnostic information may be available using the `set_option diagnostics true` command.
 ```
 This is because coercions are inserted in response to mismatched types, but a failure to synthesize an {name}`OfNat` instance is not a type mismatch.
 
@@ -354,7 +354,7 @@ def tomorrow : Later String :=
 section
 variable {α : Type u}
 ```
-:::example "Duplicate Evaluation in Coercions"
+::::example "Duplicate Evaluation in Coercions"
 Because the contents of {lean}`Coe` instances are unfolded during coercion insertion, coercions that use their argument more than once should be careful to ensure that evaluation occurs just once.
 This can be done by using a helper function that is not part of the instance, or by using {keywordOf Lean.Parser.Term.let}`let` to evaluate the coerced term and then re-use its resulting value.
 
@@ -378,15 +378,13 @@ def twice (x : α) : Twice α where
 instance : Coe α (Twice α) := ⟨twice⟩
 ```
 When the {name}`Coe` instance is unfolded, the call to {name}`twice` remains, which causes its argument to be evaluated before the body of the function is executed.
-As a result, the {keywordOf Lean.Parser.Term.dbgTrace}`dbg_trace` executes just once:
+As a result, the {keywordOf Lean.Parser.Term.dbgTrace}`dbg_trace` is included in the resulting term just once:
 ```lean (name := eval1)
 #eval ((dbg_trace "hello"; 5 : Nat) : Twice Nat)
 ```
+This used to demonstrate the effect:
 ```leanOutput eval1
 hello
-```
-```leanOutput eval1
-{ first := 5, second := 5, first_eq_second := _ }
 ```
 
 Inlining the helper into the {name}`Coe` instance results in a term that duplicates the {keywordOf Lean.Parser.Term.dbgTrace}`dbg_trace`:
@@ -400,11 +398,8 @@ instance : Coe α (Twice α) where
 hello
 hello
 ```
-```leanOutput eval2
-{ first := 5, second := 5, first_eq_second := _ }
-```
 
-Introducing an intermediate name for the result of the evaluation prevents the duplicated work:
+Introducing an intermediate name for the result of the evaluation prevents the duplication of {keywordOf Lean.Parser.Term.dbgTrace}`dbg_trace`:
 ```lean (name := eval3)
 instance : Coe α (Twice α) where
   coe x := let y := x; ⟨y, y, rfl⟩
@@ -414,11 +409,8 @@ instance : Coe α (Twice α) where
 ```leanOutput eval3
 hello
 ```
-```leanOutput eval3
-{ first := 5, second := 5, first_eq_second := _ }
-```
 
-:::
+::::
 ```lean (show := false)
 end
 ```
@@ -485,12 +477,12 @@ Non-dependent coercions are used whenever all values of the inferred type can be
 
 :::example "Defining Dependent Coercions"
 The string "four" can be coerced into the natural number {lean type:="Nat"}`4` with this instance declaration:
-````lean (name := fourCoe)
+```lean (name := fourCoe)
 instance : CoeDep String "four" Nat where
   coe := 4
 
 #eval ("four" : Nat)
-````
+```
 ```leanOutput fourCoe
 4
 ```
