Manual/Namespaces.lean
@@ -144,7 +144,10 @@ The section's name must be used to close it.
 end
 ```
 ```leanOutput english4
-invalid 'end', name is missing (expected Greetings)
+Missing name after `end`: Expected the current scope name `Greetings`
+
+Hint: To end the current scope `Greetings`, specify its name:
+  end ̲G̲r̲e̲e̲t̲i̲n̲g̲s̲
 ```
 
 ```lean
@@ -216,7 +219,7 @@ An {keywordOf Lean.Parser.Command.end}`end` command cannot close all three due t
 end A.D.E
 ```
 ```leanOutput endADE
-invalid 'end', name mismatch (expected «».D.E)
+Invalid name after `end`: Expected `D.E`, but found `A.D.E`
 ```
 Instead, namespaces and sections must be ended separately.
 ```lean
@@ -353,7 +356,8 @@ automatically included section variable(s) unused in theorem 'p_all':
   pFifteen
 consider restructuring your `variable` declarations so that the variables are not in scope or explicitly omit them:
   omit pFifteen in theorem ...
-note: this linter can be disabled with `set_option linter.unusedSectionVars false`
+
+Note: This linter can be disabled with `set_option linter.unusedSectionVars false`
 ```
 
 This can be avoided by using {keywordOf Lean.Parser.Command.omit}`omit`to remove {lean}`pFifteen`:
