Manual/Releases/v4_4_0.lean
@@ -18,7 +18,7 @@ tag := "release-v4.4.0"
 file := "v4.4.0"
 %%%
 
-`````markdown
+````markdown
 * Lake and the language server now support per-package server options using the `moreServerOptions` config field, as well as options that apply to both the language server and `lean` using the `leanOptions` config field. Setting either of these fields instead of `moreServerArgs` ensures that viewing files from a dependency uses the options for that dependency. Additionally, `moreServerArgs` is being deprecated in favor of the `moreGlobalServerArgs` field. See PR [#2858](https://github.com/leanprover/lean4/pull/2858).
 
   A Lakefile with the following deprecated package declaration:
@@ -62,4 +62,4 @@ Bug fixes for [#2628](https://github.com/leanprover/lean4/issues/2628), [#2883](
 * Later packages and libraries in the dependency tree are now preferred over earlier ones. That is, the later ones "shadow" the earlier ones. Such an ordering is more consistent with how declarations generally work in programming languages. This will break any package that relied on the previous ordering. See issue [#2548](https://github.com/leanprover/lean4/issues/2548) and PR [#2937](https://github.com/leanprover/lean4/pull/2937).
 * Executable roots are no longer mistakenly treated as importable. They will no longer be picked up by `findModule?`. See PR [#2937](https://github.com/leanprover/lean4/pull/2937).
 
-`````
+````
